Support k-invariant and so on

Analysis_More.thy
@@ -26,6 +26,11 @@ lemma has_vector_derivative_projI:
   apply (auto simp add: bounded_linear_scaleR_left)
   by (auto intro: vec_tendstoI)
 
+lemma has_vdriv_on_projI:
+  assumes "\<forall>i. ((\<lambda>t. p t $ i) has_vderiv_on (\<lambda>t. q t $ i)) D"
+  shows "(p has_vderiv_on q) D"
+  using assms has_vderiv_on_def has_vector_derivative_projI by metis
+
 lemma has_derivative_coords [simp,derivative_intros]:
   "((\<lambda>t. t$i) has_derivative (\<lambda>t. t$i)) (at x)"
   unfolding has_derivative_def by auto
@@ -461,6 +466,7 @@ proof (rule ccontr)
     by (smt "1" "10" assms(5) atLeastAtMost_iff atLeastLessThan_iff greaterThanLessThan_iff) 
 qed
 
+
 subsection \<open>Definition of states\<close>
 
 text \<open>Variable names\<close>
@@ -468,7 +474,6 @@ type_synonym var = char
 
 text \<open>State\<close>
 type_synonym state = "var \<Rightarrow> real"
-
 text \<open>Expressions\<close>
 type_synonym exp = "state \<Rightarrow> real"
 
@@ -491,8 +496,38 @@ lemma vec_state_map1[simp]: "vec2state (state2vec s) = s"
 lemma vec_state_map2[simp]: "state2vec (vec2state s) = s"
   unfolding vec2state_def state2vec_def by auto
 
-subsection \<open>Definition of ODEs\<close>
+text \<open>Conversion between state pair and vector\<close>
+definition state2vec_Pair :: "(state \<times> state) \<Rightarrow> (real^var) \<times> (real^var)"
+  where "state2vec_Pair ss = (state2vec (fst ss), state2vec (snd ss))"
 
+definition vec2state_Pair :: "(real^var) \<times> (real^var) \<Rightarrow> (state \<times> state)"
+  where "vec2state_Pair vv = (vec2state (fst vv), vec2state (snd vv))"
+
+lemma vec_state_map1_Pair[simp]: "vec2state_Pair (state2vec_Pair s) = s"
+  unfolding vec2state_Pair_def state2vec_Pair_def by auto
+
+lemma vec_state_map2_Pair[simp]: "state2vec_Pair (vec2state_Pair s) = s"
+  unfolding vec2state_Pair_def state2vec_Pair_def by auto
+
+text \<open>Conversion between k-states and vector\<close>
+
+definition state2vec_k :: "(('k :: finite) \<Rightarrow> state) \<Rightarrow> real^('k \<times> var)"
+  where "state2vec_k ss = (\<chi> x. ss (fst x) (snd x))"
+
+definition vec2state_k :: "real^(('k :: finite) \<times> char) \<Rightarrow>('k \<Rightarrow> state) "
+  where "(vec2state_k V) k v = V $ (k, v)"
+
+lemma vec_state_map1_k[simp]: "vec2state_k (state2vec_k s) = s"
+  unfolding vec2state_k_def state2vec_k_def by auto
+
+lemma vec_state_map2_k[simp]: "state2vec_k (vec2state_k s) = s"
+  unfolding vec2state_k_def state2vec_k_def by auto
+
+(*
+lemma "(\<lambda>t. state2vec_k (ps k t) $ (a, b)) = (\<lambda>t. ps k t a b)"
+*)
+
+subsection \<open>Definition of ODEs\<close>
 datatype ODE =
   ODE "var \<Rightarrow> exp"
 
@@ -500,14 +535,62 @@ text \<open>Given ODE and a state, find the derivative vector.\<close>
 fun ODE2Vec :: "ODE \<Rightarrow> state \<Rightarrow> vec" where
   "ODE2Vec (ODE f) s = state2vec (\<lambda>a. f a s)"
 
+text \<open>Given the same ODE and two state, find the derivative vector pair.\<close>
+fun ODE2Vec_Pair :: "ODE \<Rightarrow> (state \<times> state) \<Rightarrow> (real^var) \<times> (real^var)" where
+  "ODE2Vec_Pair ode ss = (ODE2Vec ode (fst ss), ODE2Vec ode (snd ss))"
+
+text \<open>Given the same ODE and k-state, find the derivative vector pair.\<close>
+fun ODE2Vec_k :: "ODE \<Rightarrow> (('k :: finite) \<Rightarrow> state) \<Rightarrow> (real^('k \<times> var))" where
+  "ODE2Vec_k (ODE f) ss = state2vec_k (\<lambda>k. \<lambda>x. f x (ss k))"
+
+
 text \<open>History p on time {0 .. d} is a solution to ode.\<close>
 definition ODEsol :: "ODE \<Rightarrow> (real \<Rightarrow> state) \<Rightarrow> real \<Rightarrow> bool" where
   "ODEsol ode p d = (d \<ge> 0 \<and> (\<exists>\<epsilon>>0. ((\<lambda>t. state2vec (p t)) has_vderiv_on (\<lambda>t. ODE2Vec ode (p t))) {-\<epsilon> .. d+\<epsilon>}))"
+
+lemma ODEsol_le: "\<lbrakk>ODEsol ode p d; t \<le> d; t \<ge> 0\<rbrakk> \<Longrightarrow> ODEsol ode p t"
+  apply (simp add: ODEsol_def)
+  by (meson add_le_cancel_right atLeastatMost_subset_iff dual_order.refl has_vderiv_on_subset)
 
 text \<open>History p on time {0 ..} is a solution to ode.\<close>
 definition ODEsolInf :: "ODE \<Rightarrow> (real \<Rightarrow> state) \<Rightarrow> bool" where
   "ODEsolInf ode p = (\<exists>\<epsilon>>0. ((\<lambda>t. state2vec (p t)) has_vderiv_on (\<lambda>t. ODE2Vec ode (p t))) {-\<epsilon> ..})"
 
+subsection \<open>More theorems about derivatives\<close>
+
+lemma has_vderiv_on_Pair:
+  assumes "(f has_vderiv_on f') S"
+      and "(g has_vderiv_on g') S"
+    shows "((\<lambda>x. (f x, g x)) has_vderiv_on (\<lambda>x. (f' x, g' x))) S"
+  using assms
+  by (auto simp: has_vderiv_on_def intro!: derivative_eq_intros)
+
+lemma derivative_exp [simp, derivative_intros]:
+  "(exp has_derivative (*) (exp (x :: real))) (at x)"
+  using DERIV_exp unfolding has_field_derivative_def
+  by auto
+
+lemma derivative_exp_const [derivative_intros]:
+  fixes c :: real
+  shows "((\<lambda>x. exp (c * x)) has_derivative (\<lambda>xa. xa * c * exp (c * x))) (at x)"
+proof-
+  have 1: "((*) c has_derivative (\<lambda>x. x * c)) (at x)"
+    apply (rule has_derivative_eq_rhs)
+     apply (auto intro!: derivative_intros)[1]
+    by auto
+  show ?thesis using has_derivative_exp[OF 1] 
+    by auto
+  qed
+
+lemma SOME_const_vderiv [derivative_intros, simp]:
+  fixes p :: " real \<Rightarrow> bool"
+  assumes "(f has_vderiv_on f') S"
+  shows "((\<lambda>t. (SOME k. p k) * f t) has_vderiv_on (\<lambda>t. (SOME k . p k) * f' t)) S"
+  apply (rule has_vderiv_on_eq_rhs)
+   apply (rule has_vderiv_on_mult)
+    apply (auto intro: derivative_intros)[1]
+  using assms apply auto
+  done
 
 subsection \<open>Further results in analysis\<close>
 
@@ -521,8 +604,42 @@ proof-
     using e(1) has_vderiv_on_subset[OF e(2)] by auto
 qed
 
+lemma ODEsol_old_Pair:
+  assumes "ODEsol ode p1 d"
+      and "ODEsol ode p2 d"
+  shows "((\<lambda>t. state2vec_Pair (p1 t, p2 t)) has_vderiv_on (\<lambda>t. ODE2Vec_Pair ode (p1 t, p2 t))) {0 .. d}"
+proof-
+  from assms have "((\<lambda>t. state2vec (p1 t)) has_vderiv_on (\<lambda>t. ODE2Vec ode (p1 t))) {0 .. d}"  
+                  "((\<lambda>t. state2vec (p2 t)) has_vderiv_on (\<lambda>t. ODE2Vec ode (p2 t))) {0 .. d}"
+    using ODEsol_old[of ode p1 d] ODEsol_old[of ode p2 d] by auto
+  then show ?thesis
+    unfolding state2vec_Pair_def
+    using has_vderiv_on_Pair[of "\<lambda>t. state2vec (p1 t)" "\<lambda>t. ODE2Vec ode (p1 t)" "{0 .. d}"
+    "\<lambda>t. state2vec (p2 t)" "\<lambda>t. ODE2Vec ode (p2 t)"]
+    by auto
+qed
+
+lemma ODEsol_old_k:
+  assumes "\<forall>k. ODEsol ode (ps k) d"
+  shows "((\<lambda>t. state2vec_k (\<lambda>k. ps k t)) has_vderiv_on (\<lambda>t. ODE2Vec_k ode (\<lambda>k. ps k t))) {0 .. d}"
+  using has_vdriv_on_projI[of "\<lambda>t. state2vec_k (\<lambda>k. ps k t)" "\<lambda>t. ODE2Vec_k ode (\<lambda>k. ps k t)" "{0..d}"]
+proof-
+  have "\<exists>f. ode = ODE f"
+    by (meson ODE.exhaust)
+  then obtain f where "ode = ODE f" 
+    by auto
+  from assms have "\<forall>k. ((\<lambda>t. state2vec (ps k t)) has_vderiv_on (\<lambda>t. ODE2Vec ode (ps k t))) {0 .. d}"
+    using ODEsol_old by blast
+  then have "\<forall>k i. ((\<lambda>x. ps k x i) has_vderiv_on (\<lambda>x. f i (ps k x))) {0..d}"
+    using ODE2Vec.simps \<open>ode = ODE f\<close> has_vderiv_on_proj state2vec_def by fastforce
+  then show ?thesis
+    using has_vdriv_on_projI[of "\<lambda>t. state2vec_k (\<lambda>k. ps k t)" "\<lambda>t. ODE2Vec_k ode (\<lambda>k. ps k t)" "{0..d}"]
+    \<open>ode = ODE f\<close> state2vec_k_def 
+    by (smt (z3) ODE2Vec_k.simps has_vderiv_on_def has_vector_derivative_transform vec_lambda_beta)
+qed
+
 lemma ODEsolInf_old:
-   assumes "ODEsolInf  ode p"
+   assumes "ODEsolInf ode p"
    shows "((\<lambda>t. state2vec (p t)) has_vderiv_on (\<lambda>t. ODE2Vec ode (p t))) {0 ..}"
 proof-
   obtain e where e: "e > 0" "((\<lambda>t. state2vec (p t)) has_vderiv_on (\<lambda>t. ODE2Vec ode (p t))) {-e ..}"
