hhl/BigStepSimple.thy
@@ -1,0 +1,448 @@
+theory BigStepSimple
+  imports "../Language"
+begin
+
+subsection \<open>Validity\<close>
+
+text \<open>Assertion is a predicate on states and traces\<close>
+
+type_synonym assn = "state \<Rightarrow> trace \<Rightarrow> bool"
+
+definition Valid :: "assn \<Rightarrow> proc \<Rightarrow> assn \<Rightarrow> bool" ("\<Turnstile>\<^sub>H\<^sub>L ({(1_)}/ (_)/ {(1_)})" 50) where
+  "\<Turnstile>\<^sub>H\<^sub>L {P} c {Q} \<longleftrightarrow> (\<forall>s1 tr1 s2 tr2. P s1 tr1 \<longrightarrow> big_step c s1 tr2 s2 \<longrightarrow> Q s2 (tr1 @ tr2))"
+
+definition entails :: "assn \<Rightarrow> assn \<Rightarrow> bool" (infixr "\<Longrightarrow>\<^sub>A" 25) where
+  "(P \<Longrightarrow>\<^sub>A Q) \<longleftrightarrow> (\<forall>s tr. P s tr \<longrightarrow> Q s tr)"
+
+lemma entails_refl [simp]:
+  "P \<Longrightarrow>\<^sub>A P"
+  unfolding entails_def by auto
+
+lemma entails_trans:
+  "(P \<Longrightarrow>\<^sub>A Q) \<Longrightarrow> (Q \<Longrightarrow>\<^sub>A R) \<Longrightarrow> (P \<Longrightarrow>\<^sub>A R)"
+  unfolding entails_def by auto
+
+lemma Valid_ex_pre:
+  "(\<And>v. \<Turnstile>\<^sub>H\<^sub>L {P v} c {Q}) \<Longrightarrow> \<Turnstile>\<^sub>H\<^sub>L {\<lambda>s t. \<exists>v. P v s t} c {Q}"
+  unfolding Valid_def by auto
+
+lemma Valid_ex_post:
+  "\<exists>v. \<Turnstile>\<^sub>H\<^sub>L {P} c {Q v} \<Longrightarrow> \<Turnstile>\<^sub>H\<^sub>L {P} c {\<lambda>s t. \<exists>v. Q v s t}"
+  unfolding Valid_def by blast
+
+lemma Valid_and_pre:
+  "(P1 \<Longrightarrow> \<Turnstile>\<^sub>H\<^sub>L {P} c {Q}) \<Longrightarrow> \<Turnstile>\<^sub>H\<^sub>L {\<lambda>s t. P1 \<and> P s t} c {Q}"
+  unfolding Valid_def by auto
+
+theorem Valid_weaken_pre:
+  "P \<Longrightarrow>\<^sub>A P' \<Longrightarrow> \<Turnstile>\<^sub>H\<^sub>L {P'} c {Q} \<Longrightarrow> \<Turnstile>\<^sub>H\<^sub>L {P} c {Q}"
+  unfolding Valid_def entails_def by blast
+
+theorem Valid_strengthen_post:
+  "Q \<Longrightarrow>\<^sub>A Q' \<Longrightarrow> \<Turnstile>\<^sub>H\<^sub>L {P} c {Q} \<Longrightarrow> \<Turnstile>\<^sub>H\<^sub>L {P} c {Q'}"
+  unfolding Valid_def entails_def by blast
+
+theorem Valid_skip:
+  "\<Turnstile>\<^sub>H\<^sub>L {P} Skip {P}"
+  unfolding Valid_def
+  by (auto elim: skipE)
+
+theorem Valid_assign:
+  "\<Turnstile>\<^sub>H\<^sub>L {\<lambda>s. Q (s(var := e s))} var ::= e {Q}"
+  unfolding Valid_def
+  by (auto elim: assignE)
+
+theorem Valid_havoc:
+  "\<Turnstile>\<^sub>H\<^sub>L {\<lambda>s tr. \<forall>v. Q (s(var := v)) tr} var ::= * {Q}"
+  unfolding Valid_def
+  by (auto elim: HavocE)
+
+theorem Valid_assume:
+  "\<Turnstile>\<^sub>H\<^sub>L {\<lambda>s tr. b s \<longrightarrow> Q s tr} Assume b {Q}"
+  unfolding Valid_def
+  by (auto elim: AssumeE)
+
+theorem Valid_send:
+  "\<Turnstile>\<^sub>H\<^sub>L {\<lambda>s tr. Q s (tr @ [OutBlock ch (e s)]) \<and>
+              (\<forall>d::real>0. Q s (tr @ [WaitBlk d (\<lambda>_. State s) ({ch}, {}), OutBlock ch (e s)])) \<and>
+              Q s (tr @ [WaitBlk \<infinity> (\<lambda>_. State s) ({ch}, {})])}
+       Cm (ch[!]e) {Q}"
+  unfolding Valid_def
+  by (auto elim: sendE)
+
+theorem Valid_receive:
+  "\<Turnstile>\<^sub>H\<^sub>L {\<lambda>s tr. (\<forall>v. Q (s(var := v)) (tr @ [InBlock ch v])) \<and>
+              (\<forall>d::real>0. \<forall>v. Q (s(var := v))
+                (tr @ [WaitBlk d (\<lambda>_. State s) ({}, {ch}), InBlock ch v])) \<and>
+              Q s (tr @ [WaitBlk \<infinity> (\<lambda>_. State s) ({}, {ch})])}
+       Cm (ch[?]var) {Q}"
+  unfolding Valid_def
+  by (auto elim: receiveE)
+
+theorem Valid_seq:
+  "\<Turnstile>\<^sub>H\<^sub>L {P} c1 {Q} \<Longrightarrow> \<Turnstile>\<^sub>H\<^sub>L {Q} c2 {R} \<Longrightarrow> \<Turnstile>\<^sub>H\<^sub>L {P} c1; c2 {R}"
+  unfolding Valid_def
+  apply (auto elim!: seqE) by fastforce
+
+theorem Valid_rep:
+  assumes "\<Turnstile>\<^sub>H\<^sub>L {P} c {P}"
+  shows "\<Turnstile>\<^sub>H\<^sub>L {P} Rep c {P}"
+proof -
+  have "big_step p s1 tr2 s2 \<Longrightarrow> p = Rep c \<Longrightarrow> \<forall>tr1. P s1 tr1 \<longrightarrow> P s2 (tr1 @ tr2)" for p s1 s2 tr2
+    apply (induct rule: big_step.induct, auto)
+    by (metis Valid_def append.assoc assms)
+  then show ?thesis
+    using assms unfolding Valid_def by auto
+qed
+
+theorem Valid_ichoice:
+  assumes "\<Turnstile>\<^sub>H\<^sub>L {P1} c1 {Q}"
+    and "\<Turnstile>\<^sub>H\<^sub>L {P2} c2 {Q}"
+  shows "\<Turnstile>\<^sub>H\<^sub>L {\<lambda>s tr. P1 s tr \<and> P2 s tr} IChoice c1 c2 {Q}"
+  using assms unfolding Valid_def by (auto elim: ichoiceE)
+
+theorem Valid_ichoice_sp:
+  assumes "\<Turnstile>\<^sub>H\<^sub>L {P} c1 {Q1}"
+    and "\<Turnstile>\<^sub>H\<^sub>L {P} c2 {Q2}"
+  shows "\<Turnstile>\<^sub>H\<^sub>L {P} IChoice c1 c2 {\<lambda>s tr. Q1 s tr \<or> Q2 s tr}"
+  using assms unfolding Valid_def by (auto elim: ichoiceE)
+
+
+subsection \<open>Assertions on traces\<close>
+type_synonym tassn = "trace \<Rightarrow> bool"
+
+definition entails_tassn :: "tassn \<Rightarrow> tassn \<Rightarrow> bool" (infixr "\<Longrightarrow>\<^sub>t" 25) where
+  "(P \<Longrightarrow>\<^sub>t Q) \<longleftrightarrow> (\<forall>tr. P tr \<longrightarrow> Q tr)"
+
+lemma entails_tassn_refl [simp]:
+  "P \<Longrightarrow>\<^sub>t P"
+  unfolding entails_tassn_def by auto
+
+lemma entails_tassn_trans:
+  "(P \<Longrightarrow>\<^sub>t Q) \<Longrightarrow> (Q \<Longrightarrow>\<^sub>t R) \<Longrightarrow> (P \<Longrightarrow>\<^sub>t R)"
+  unfolding entails_tassn_def by auto
+
+lemma entails_tassn_ex_pre:
+  "(\<And>x. P x \<Longrightarrow>\<^sub>t Q) \<Longrightarrow> (\<lambda>tr. (\<exists>x. P x tr)) \<Longrightarrow>\<^sub>t Q"
+  by (auto simp add: entails_tassn_def)
+
+lemma entails_tassn_ex_post:
+  "(\<exists>x. P \<Longrightarrow>\<^sub>t Q x) \<Longrightarrow> P \<Longrightarrow>\<^sub>t (\<lambda>tr. (\<exists>x. Q x tr))"
+  by (auto simp add: entails_tassn_def)
+
+definition emp_assn :: "tassn" ("emp\<^sub>t") where
+  "emp\<^sub>t = (\<lambda>tr. tr = [])"
+
+definition join_assn :: "tassn \<Rightarrow> tassn \<Rightarrow> tassn" (infixr "@\<^sub>t" 65) where
+  "P @\<^sub>t Q = (\<lambda>tr. \<exists>tr1 tr2. P tr1 \<and> Q tr2 \<and> tr = tr1 @ tr2)"
+
+definition magic_wand_assn :: "tassn \<Rightarrow> tassn \<Rightarrow> tassn" (infixr "@-" 65) where
+  "Q @- P = (\<lambda>tr. \<forall>tr1. Q tr1 \<longrightarrow> P (tr @ tr1))"
+
+definition all_assn :: "('a \<Rightarrow> tassn) \<Rightarrow> tassn" (binder "\<forall>\<^sub>t" 10) where
+  "(\<forall>\<^sub>tv. P v) = (\<lambda>tr. \<forall>v. P v tr)"
+
+definition ex_assn :: "('a \<Rightarrow> tassn) \<Rightarrow> tassn" (binder "\<exists>\<^sub>t" 10) where
+  "(\<exists>\<^sub>tv. P v) = (\<lambda>tr. \<exists>v. P v tr)"
+
+definition conj_assn :: "tassn \<Rightarrow> tassn \<Rightarrow> tassn" (infixr "\<and>\<^sub>t" 35) where
+  "(P \<and>\<^sub>t Q) = (\<lambda>tr. P tr \<and> Q tr)"
+
+definition disj_assn :: "tassn \<Rightarrow> tassn \<Rightarrow> tassn" (infixr "\<or>\<^sub>t" 25) where
+  "(P \<or>\<^sub>t Q) = (\<lambda>tr. P tr \<or> Q tr)"
+
+definition imp_assn :: "tassn \<Rightarrow> tassn \<Rightarrow> tassn" (infixr "\<longrightarrow>\<^sub>t" 25) where
+  "(P \<longrightarrow>\<^sub>t Q) = (\<lambda>tr. P tr \<longrightarrow> Q tr)"
+
+definition pure_assn :: "bool \<Rightarrow> tassn" ("\<up>") where
+  "\<up>b = (\<lambda>_. b)"
+
+inductive out_assn :: "gstate \<Rightarrow> cname \<Rightarrow> real \<Rightarrow> tassn" ("Out\<^sub>t") where
+  "Out\<^sub>t s ch v [OutBlock ch v]"
+| "(d::real) > 0 \<Longrightarrow> Out\<^sub>t s ch v [WaitBlk (ereal d) (\<lambda>_. s) ({ch}, {}), OutBlock ch v]"
+| "Out\<^sub>t s ch v [WaitBlk \<infinity> (\<lambda>_. s) ({ch}, {})]"
+
+inductive in_assn :: "gstate \<Rightarrow> cname \<Rightarrow> real \<Rightarrow> tassn" ("In\<^sub>t") where
+  "In\<^sub>t s ch v [InBlock ch v]"
+| "(d::real) > 0 \<Longrightarrow> In\<^sub>t s ch v [WaitBlk (ereal d) (\<lambda>_. s) ({}, {ch}), InBlock ch v]"
+| "In\<^sub>t s ch v [WaitBlk \<infinity> (\<lambda>_. s) ({}, {ch})]"
+
+inductive io_assn :: "cname \<Rightarrow> real \<Rightarrow> tassn" ("IO\<^sub>t") where
+  "IO\<^sub>t ch v [IOBlock ch v]"
+
+inductive wait_assn :: "real \<Rightarrow> (real \<Rightarrow> gstate) \<Rightarrow> rdy_info \<Rightarrow> tassn" ("Wait\<^sub>t") where
+  "d > 0 \<Longrightarrow> Wait\<^sub>t d p rdy [WaitBlk d (\<lambda>\<tau>. p \<tau>) rdy]"
+| "d \<le> 0 \<Longrightarrow> Wait\<^sub>t d p rdy []"
+
+lemma emp_unit_left [simp]:
+  "(emp\<^sub>t @\<^sub>t P) = P"
+  unfolding join_assn_def emp_assn_def by auto
+
+lemma emp_unit_right [simp]:
+  "(P @\<^sub>t emp\<^sub>t) = P"
+  unfolding join_assn_def emp_assn_def by auto
+
+lemma emp_unit_right':
+  "P = (P @\<^sub>t emp\<^sub>t) "
+  unfolding join_assn_def emp_assn_def by auto
+
+lemma join_assoc:
+  "(P @\<^sub>t Q) @\<^sub>t R = P @\<^sub>t (Q @\<^sub>t R)"
+  unfolding join_assn_def by fastforce
+
+lemma entails_mp_emp:
+  "emp\<^sub>t \<Longrightarrow>\<^sub>t P @- P"
+  unfolding entails_tassn_def emp_assn_def magic_wand_assn_def by auto
+
+lemma entails_mp:
+  "Q \<Longrightarrow>\<^sub>t P @- (Q @\<^sub>t P)"
+  unfolding entails_tassn_def magic_wand_assn_def join_assn_def by auto
+
+lemma magic_wand_mono:
+  "P \<Longrightarrow>\<^sub>t Q \<Longrightarrow> (R @- P) \<Longrightarrow>\<^sub>t (R @- Q)"
+  unfolding entails_tassn_def magic_wand_assn_def by auto
+
+definition false_assn :: "tassn" ("false\<^sub>A") where
+  "false_assn tr = False"
+
+lemma false_assn_entails [simp]:
+  "false\<^sub>A \<Longrightarrow>\<^sub>t P"
+  by (simp add: entails_tassn_def false_assn_def)
+
+lemma pure_assn_entails [simp]:
+  "(\<up>b \<and>\<^sub>t P \<Longrightarrow>\<^sub>t Q) = (b \<longrightarrow> P \<Longrightarrow>\<^sub>t Q)"
+  unfolding entails_tassn_def conj_assn_def pure_assn_def by auto
+
+lemma entails_tassn_cancel_left:
+  "Q \<Longrightarrow>\<^sub>t R \<Longrightarrow> P @\<^sub>t Q \<Longrightarrow>\<^sub>t P @\<^sub>t R"
+  by (auto simp add: entails_tassn_def join_assn_def)
+
+lemma entails_tassn_cancel_left_emp:
+  "Q \<Longrightarrow>\<^sub>t emp\<^sub>t  \<Longrightarrow> P @\<^sub>t Q \<Longrightarrow>\<^sub>t P "
+  by (auto simp add: entails_tassn_def join_assn_def emp_assn_def)
+
+lemma entails_tassn_cancel_right:
+  "P \<Longrightarrow>\<^sub>t Q \<Longrightarrow> P @\<^sub>t R \<Longrightarrow>\<^sub>t Q @\<^sub>t R"
+  by (auto simp add: entails_tassn_def join_assn_def)
+
+lemma entails_tassn_cancel_both:
+  "P \<Longrightarrow>\<^sub>t Q \<Longrightarrow> R \<Longrightarrow>\<^sub>t S \<Longrightarrow> P @\<^sub>t R \<Longrightarrow>\<^sub>t Q @\<^sub>t S"
+  by (auto simp add: entails_tassn_def join_assn_def)
+
+lemma entails_tassn_conj:
+  "P \<Longrightarrow>\<^sub>t Q \<Longrightarrow> P \<Longrightarrow>\<^sub>t R \<Longrightarrow> P \<Longrightarrow>\<^sub>t (Q \<and>\<^sub>t R)"
+  by (auto simp add: entails_tassn_def conj_assn_def)
+
+lemma entails_tassn_exI:
+  "P \<Longrightarrow>\<^sub>t Q x \<Longrightarrow> P \<Longrightarrow>\<^sub>t (\<exists>\<^sub>t x. Q x)"
+  unfolding ex_assn_def entails_tassn_def by auto
+
+lemma conj_join_distrib [simp]:
+  "(\<up>b \<and>\<^sub>t P) @\<^sub>t Q = (\<up>b \<and>\<^sub>t (P @\<^sub>t Q))"
+  by (auto simp add: join_assn_def conj_assn_def pure_assn_def)
+
+lemma conj_join_distrib2 [simp]:
+  "(\<lambda>tr. b \<and> P tr) @\<^sub>t Q = (\<up>b \<and>\<^sub>t (P @\<^sub>t Q))"
+  by (auto simp add: pure_assn_def conj_assn_def join_assn_def)
+
+lemma wait_le_zero [simp]:
+  "d \<le> 0 \<Longrightarrow> Wait\<^sub>t d p rdy = emp\<^sub>t"
+  apply (rule ext) subgoal for tr
+    apply auto
+     apply (cases rule: wait_assn.cases)
+    apply (auto simp add: emp_assn_def)
+    by (auto intro: wait_assn.intros)
+  done
+
+text \<open>Simpler forms of weakest precondition\<close>
+
+theorem Valid_send':
+  "\<Turnstile>\<^sub>H\<^sub>L {\<lambda>s. Out\<^sub>t (State s) ch (e s) @- Q s}
+       Cm (ch[!]e)
+      {Q}"
+  apply (rule Valid_weaken_pre)
+   prefer 2 apply (rule Valid_send)
+  unfolding entails_def magic_wand_assn_def
+  by (auto intro: out_assn.intros)
+
+theorem Valid_receive':
+  "\<Turnstile>\<^sub>H\<^sub>L {\<lambda>s. \<forall>\<^sub>tv. In\<^sub>t (State s) ch v @- Q (s(var := v))}
+       Cm (ch[?]var)
+      {Q}"
+  apply (rule Valid_weaken_pre)
+   prefer 2 apply (rule Valid_receive)
+  unfolding entails_def magic_wand_assn_def all_assn_def
+  by (metis fun_upd_triv in_assn.intros)
+
+text \<open>Strongest postcondition forms\<close>
+
+theorem Valid_assign_sp:
+  "\<Turnstile>\<^sub>H\<^sub>L {\<lambda>s t. P s t}
+       Assign var e
+      {\<lambda>s t. \<exists>x. s var = e (s(var := x)) \<and> P (s(var := x)) t}"
+  apply (rule Valid_weaken_pre)
+   prefer 2 apply (rule Valid_assign)
+  apply (auto simp add: entails_def)
+  subgoal for s tr
+    apply (rule exI[where x="s var"])
+    by auto
+  done
+
+theorem Valid_havoc_sp:
+  "\<Turnstile>\<^sub>H\<^sub>L {\<lambda>s t. P s t}
+       Havoc var 
+      {\<lambda>s t. \<exists>x. P (s(var := x)) t}"
+  apply (rule Valid_weaken_pre)
+   prefer 2 apply (rule Valid_havoc)
+  apply (auto simp add: entails_def)
+  subgoal for s tr
+    by (metis fun_upd_triv)
+  done
+
+theorem Valid_send_sp:
+  "\<Turnstile>\<^sub>H\<^sub>L {\<lambda>s t. P s t}
+       Cm (ch[!]e)
+     {\<lambda>s t. (P s @\<^sub>t Out\<^sub>t (State s) ch (e s)) t}"
+  apply (rule Valid_weaken_pre)
+   prefer 2 apply (rule Valid_send')
+  by (auto simp add: entails_def magic_wand_assn_def join_assn_def)
+
+theorem Valid_receive_sp:
+  "\<Turnstile>\<^sub>H\<^sub>L {\<lambda>s t. P s t}
+       Cm (ch[?]var)
+      {\<lambda>s t. \<exists>x v. (\<up>(s var = v) \<and>\<^sub>t (P(s(var := x)) @\<^sub>t In\<^sub>t (State (s(var := x))) ch v)) t}"
+  apply (rule Valid_weaken_pre)
+   prefer 2 apply (rule Valid_receive)
+  unfolding entails_def
+  apply (auto simp add: join_assn_def)
+  subgoal for s tr v
+    apply (rule exI[where x="s var"])
+    apply (rule exI[where x=v])
+    apply (auto simp add: conj_assn_def pure_assn_def)
+    apply (rule exI[where x=tr]) by (auto intro: in_assn.intros)
+  subgoal for s tr d v
+    apply (rule exI[where x="s var"])
+    apply (rule exI[where x=v])
+    apply (auto simp add: conj_assn_def pure_assn_def)
+    apply (rule exI[where x=tr])
+    apply auto apply (rule in_assn.intros) by auto
+  subgoal for s tr
+    apply (rule exI[where x="s var"])
+    apply (auto simp add: conj_assn_def pure_assn_def)
+    apply (rule exI[where x=tr])
+    apply auto by (rule in_assn.intros)
+  done
+
+theorem Valid_assume_sp:
+   "\<Turnstile>\<^sub>H\<^sub>L {\<lambda>s t. P s t} Assume b {\<lambda>s t. b s \<and> P s t}"
+  unfolding Valid_def
+  by (metis AssumeE self_append_conv)
+
+theorem Valid_if_split:
+  assumes "b \<Longrightarrow> \<Turnstile>\<^sub>H\<^sub>L {P1} c {Q1}"
+    and "\<not>b \<Longrightarrow> \<Turnstile>\<^sub>H\<^sub>L {P2} c {Q2}"
+  shows "\<Turnstile>\<^sub>H\<^sub>L {\<lambda>s t. if b then P1 s t else P2 s t}
+             c
+            {\<lambda>s t. if b then Q1 s t else Q2 s t}"
+  using assms unfolding Valid_def
+  by auto
+
+theorem Valid_assign_sp_st:
+  "\<Turnstile>\<^sub>H\<^sub>L {\<lambda>s t. s = st \<and> P s t}
+        x ::= e
+      {\<lambda>s t. s = st(x := e st) \<and> P st t}"
+  apply (rule Valid_weaken_pre)
+   prefer 2 apply (rule Valid_assign)
+  by (auto simp add: entails_def)
+
+theorem Valid_havoc_sp_st:
+  "\<Turnstile>\<^sub>H\<^sub>L {\<lambda>s t. s = st \<and> P s t}
+        x ::= *
+      {\<lambda>s t. \<exists>v. s = st(x := v) \<and> P st t}"
+  apply (rule Valid_weaken_pre)
+   prefer 2 apply (rule Valid_havoc)
+  by (auto simp add: entails_def)
+
+theorem Valid_assign_sp_bst:
+  "\<Turnstile>\<^sub>H\<^sub>L {\<lambda>s t. s = st \<and> b s \<and> P s t}
+        x ::= *
+      {\<lambda>s t. \<exists>v. s = st(x := v) \<and> b st \<and> P st t}"
+  apply (rule Valid_weaken_pre)
+   prefer 2 apply (rule Valid_havoc)
+  by (auto simp add: entails_def)
+
+theorem Valid_send_sp_st:
+  "\<Turnstile>\<^sub>H\<^sub>L {\<lambda>s t. s = st \<and> P s t}
+       Cm (ch[!]e)
+      {\<lambda>s t. s = st \<and> (P st @\<^sub>t Out\<^sub>t (State st) ch (e st)) t}"
+  apply (rule Valid_weaken_pre)
+   prefer 2 apply (rule Valid_send')
+  by (auto simp add: entails_def magic_wand_assn_def join_assn_def)
+
+theorem Valid_send_sp_bst:
+  "\<Turnstile>\<^sub>H\<^sub>L {\<lambda>s t. s = st \<and> b s \<and> P s t}
+       Cm (ch[!]e)
+      {\<lambda>s t. s = st \<and> b s \<and> (P st @\<^sub>t Out\<^sub>t (State st) ch (e st)) t}"
+  apply (rule Valid_weaken_pre)
+   prefer 2 apply (rule Valid_send')
+  by (auto simp add: entails_def magic_wand_assn_def join_assn_def)
+
+theorem Valid_receive_sp_st:
+  "\<Turnstile>\<^sub>H\<^sub>L {\<lambda>s t. s = st \<and> P s t}
+        Cm (ch[?]var)
+      {\<lambda>s t. \<exists>v. s = st(var := v) \<and> (P st @\<^sub>t In\<^sub>t (State st) ch v) t}"
+  apply (rule Valid_weaken_pre)
+   prefer 2 apply (rule Valid_receive)
+  unfolding entails_def
+  apply (auto simp add: all_assn_def magic_wand_assn_def emp_assn_def join_assn_def)
+  subgoal for tr v
+    apply (rule exI[where x=v])
+    apply auto apply (rule exI[where x=tr])
+    by (simp add: in_assn.intros)
+  subgoal for tr d v
+    apply (rule exI[where x=v])
+    apply auto apply (rule exI[where x=tr])
+    using in_assn.intros(2) by auto
+  subgoal for tr
+    apply (rule exI[where x="st var"])
+    apply auto apply (rule exI[where x=tr])
+    by (metis in_assn.intros(3) infinity_ereal_def)
+  done
+
+theorem Valid_receive_sp_bst:
+  "\<Turnstile>\<^sub>H\<^sub>L {\<lambda>s t. s = st \<and> b s \<and> P s t}
+        Cm (ch[?]var)
+      {\<lambda>s t. \<exists>v. s = st(var := v) \<and> b st \<and> (P st @\<^sub>t In\<^sub>t (State st) ch v) t}"
+  apply (rule Valid_weaken_pre)
+   prefer 2 apply (rule Valid_receive)
+  unfolding entails_def
+  apply (auto simp add: all_assn_def magic_wand_assn_def emp_assn_def join_assn_def)
+  subgoal for tr v
+    apply (rule exI[where x=v])
+    apply auto apply (rule exI[where x=tr])
+    by (simp add: in_assn.intros)
+  subgoal for tr d v
+    apply (rule exI[where x=v])
+    apply auto apply (rule exI[where x=tr])
+    using in_assn.intros(2) by auto
+  subgoal for tr
+    apply (rule exI[where x="st var"])
+    apply auto apply (rule exI[where x=tr])
+    by (metis in_assn.intros(3) infinity_ereal_def)
+  done
+
+
+subsection \<open>Rules for internal and external choice\<close>
+
+text \<open>Additional assertions\<close>
+
+inductive inrdy_assn :: "state \<Rightarrow> cname \<Rightarrow> real \<Rightarrow> rdy_info \<Rightarrow> tassn" ("Inrdy\<^sub>t") where
+  "Inrdy\<^sub>t s ch v rdy [InBlock ch v]"
+| "(d::real) > 0 \<Longrightarrow> Inrdy\<^sub>t s ch v rdy [WaitBlk d (\<lambda>_. State s) rdy, InBlock ch v]"
+
+inductive outrdy_assn :: "state \<Rightarrow> cname \<Rightarrow> real \<Rightarrow> rdy_info \<Rightarrow> tassn" ("Outrdy\<^sub>t") where
+  "Outrdy\<^sub>t s ch v rdy [OutBlock ch v]"
+| "(d::real) > 0 \<Longrightarrow> Outrdy\<^sub>t s ch v rdy [WaitBlk d (\<lambda>_. State s) rdy, OutBlock ch v]"
+
+
+end
